FOL/NV/Sub/Prop/All/Rec/Sub.lean
@@ -93,7 +93,7 @@ lemma sub_no_predVar
 
 theorem substitution_theorem
   (D : Type)
-  (I : Interpretation D)
+  (I : Interpretation_ D)
   (V : Valuation_ D)
   (E : Env)
   (τ : PredName → PredName)
