FOL/NV/Sub/Var/All/Ind/Sub.lean
@@ -128,7 +128,7 @@ def IsSub (σ : VarName → VarName) (F F' : Formula) : Prop := IsSubAux σ ∅ 
 
 theorem substitution_theorem_aux
   (D : Type)
-  (I : Interpretation D)
+  (I : Interpretation_ D)
   (V V' : Valuation_ D)
   (E : Env)
   (σ : VarName → VarName)
@@ -275,7 +275,7 @@ theorem substitution_theorem_aux
 
 theorem substitution_theorem
   (D : Type)
-  (I : Interpretation D)
+  (I : Interpretation_ D)
   (V : Valuation_ D)
   (E : Env)
   (σ : VarName → VarName)
