FOL/NV/Sub/Var/All/Rec/Admits.lean
@@ -73,7 +73,7 @@ instance
 
 theorem substitution_theorem_aux
   (D : Type)
-  (I : Interpretation D)
+  (I : Interpretation_ D)
   (V V' : Valuation_ D)
   (E : Env)
   (σ σ' : VarName → VarName)
@@ -208,7 +208,7 @@ theorem substitution_theorem_aux
 
 theorem substitution_theorem
   (D : Type)
-  (I : Interpretation D)
+  (I : Interpretation_ D)
   (V : Valuation_ D)
   (E : Env)
   (σ : VarName → VarName)
